split phi away

src/tls/experiments/ConnectionTable/ConnectionTable.fsti
@@ -1,6 +1,6 @@
 module ConnectionTable
+include ConnectionTable_Aux
 
-open FStar.ReflexiveTransitiveClosure
 open FStar.Monotonic.DependentMap
 
 open FStar.HyperStack
@@ -13,8 +13,6 @@ module B = LowStar.Buffer
 module AEAD = Crypto.AEAD
 module AE = Crypto.AE
 module EE = EverCrypt.Error
-
-open ConnectionTable_Aux
 
 (*
   The connection table and ids are model artifacts that do not exist
@@ -58,38 +56,6 @@ open ConnectionTable_Aux
       state: t {token_p st (fun h -> nonce_of st h == nonce)}
 *)
 
-let model = Flags.model && Flags.ideal_AEAD
-
-let maybe_id = if model then connection_id else unit
-
-noeq
-type connection =
-  | Init: cfg:configuration -> connection
-  | Sent_HRR: ch:client_hello -> connection
-  | Sent_ServerHello: ch:client_hello -> id1:maybe_id -> connection
-  | Complete: ch:client_hello -> id1:maybe_id -> connection
-
-let step (s1 s2:connection) : Type0 =
-  match s1, s2 with
-  | Init _, Sent_HRR _ -> True
-  | Init _, Sent_ServerHello _ _ -> True
-  | Sent_ServerHello ch id1, Complete ch' id1' -> ch == ch' /\ id1 == id1'
-  | _, _ -> False
-
-let rel : Preorder.preorder connection = closure step
-
-// Store the ID rather than making it a parameter?
-let connection_ref (id:maybe_id) = 
-  r:mmmref connection rel{frameOf r `extends` rgn}
-
-val minv: partial_dependent_map maybe_id connection_ref -> Type0
-
-unfold
-let _connection_table = t rgn maybe_id connection_ref minv
-
-unfold
-let connection_table = if model then _connection_table else unit
-
 inline_for_extraction noextract
 val empty: m:imap maybe_id connection_ref minv{m == T.empty}
 
@@ -116,21 +82,9 @@ val alloc: unit -> ST connection_table
 
 val table : connection_table 
 
-let phi s = 
-  Seq.length s >= 32 /\
-  (if model then
-    let random = Seq.slice s 0 32 in
-    let id = id_of_random random in
-    let t:_connection_table = table in
-    token_p t (fun h -> 
-      T.defined t id h /\
-      (let c = T.value_of t id h in
-      token_p c (fun h' -> 
-        Sent_HRR? (sel h' c) /\
-        CH1 random == Sent_HRR?.ch (sel h' c))))
-   else True)
+let cookie_phi = cookie_phi table
 
-val cookie_key : k:option (AE.state alg phi){
+val cookie_key : k:option (AE.state alg cookie_phi){
   Some? k ==>
     (let k = Some?.v k in 
      (model ==> AE.safe k) /\
