src/tls/experiments/ConnectionTable/ConnectionTable_Aux.fst
@@ -2,15 +2,20 @@ module ConnectionTable_Aux
 
 module AE = Crypto.AEAD
 module B = LowStar.Buffer
+module T = FStar.Monotonic.DependentMap
+module DM = FStar.DependentMap
+module S = Spec.Agile.AEAD
+module HS = FStar.HyperStack
+module HST = FStar.HyperStack.ST
 
 let connection_id = UInt8.t
 
 let configuration = UInt32.t
 
-let alg = Spec.AEAD.AES128_GCM
+let alg = S.AES128_GCM
 
 let cookie = c:AE.cipher_p alg
-  {B.length c == 64 + AE.iv_length + Spec.AEAD.tag_length alg}
+  {B.length c == 64 + AE.iv_length + S.tag_length alg}
 
 let cookie_rgn = Mem.tls_define_region
 let table_rgn  = Mem.tls_tables_region
@@ -44,3 +49,53 @@ val ch_compatible: ch:client_hello -> cfg:configuration -> bool
 let ch_compatible ch cfg = false
 
 let rgn = table_rgn
+
+let model = Flags.model && Flags.ideal_AEAD
+
+let maybe_id = if model then connection_id else unit
+
+noeq
+type connection =
+  | Init: cfg:configuration -> connection
+  | Sent_HRR: ch:client_hello -> connection
+  | Sent_ServerHello: ch:client_hello -> id1:maybe_id -> connection
+  | Complete: ch:client_hello -> id1:maybe_id -> connection
+
+let step (s1 s2:connection) : Type0 =
+  match s1, s2 with
+  | Init _, Sent_HRR _ -> True
+  | Init _, Sent_ServerHello _ _ -> True
+  | Sent_ServerHello ch id1, Complete ch' id1' -> ch == ch' /\ id1 == id1'
+  | _, _ -> False
+
+let rel : Preorder.preorder connection = FStar.ReflexiveTransitiveClosure.closure step
+
+// Store the ID rather than making it a parameter?
+let connection_ref (id:maybe_id) = 
+  r:HST.mmmref connection rel{HS.frameOf r `HS.extends` rgn}
+
+// References to connections live in pairwise disjoint regions
+let minv (m:T.partial_dependent_map maybe_id connection_ref) =
+  forall id1 id2.{:pattern (Some? (DM.sel m id1)); (Some? (DM.sel m id2))}
+    (id1 <> id2 /\ Some? (DM.sel m id1) /\ Some? (DM.sel m id2)) ==>
+    HS.frameOf (Some?.v (DM.sel m id1)) `HS.disjoint` HS.frameOf (Some?.v (DM.sel m id2))
+
+unfold
+let _connection_table = T.t rgn maybe_id connection_ref minv
+
+unfold
+let connection_table = if model then _connection_table else unit
+
+let cookie_phi (table: connection_table) s = 
+  Seq.length s >= 32 /\
+  (if model then
+    let random = Seq.slice s 0 32 in
+    let id = id_of_random random in
+    let t:_connection_table = table in
+    HST.token_p t (fun h -> 
+      T.defined t id h /\
+      (let c = T.value_of t id h in
+      HST.token_p c (fun h' -> 
+        Sent_HRR? (HS.sel h' c) /\
+        CH1 random == Sent_HRR?.ch (HS.sel h' c))))
+   else True)
